terminaison (store_pointer_pair / ll_order)
git-svn-id: https://www.lri.fr/svn/demons/why2/trunk@866 ecafba89-7d34-45a1-8a0b-92829e960b72

examples-c/linked-lists/list.h
@@ -15,3 +15,5 @@ typedef struct struct_list {
 /*@ predicate eq_list(plist l1, plist l2) */
 /*@ predicate disjoint(plist l1, plist l2) */
 
+/*@ logic StorePointerPair store_pointer_pair(list l) reads l->tl */
+
